Updates.

FOL/Computing/DFS.lean
@@ -17,6 +17,7 @@ abbrev Graph
 
 /--
   `nexts g x` := The image of `x` under `g`. The neighbors of `x`.
+  `nexts g x = {y | (x, y) ∈ g}`
 -/
 def nexts
   {Node : Type}
@@ -416,7 +417,8 @@ def relation_image
   {α : Type}
   [DecidableEq α]
   (r : Set (α × α))
-  (S : Set α) :=
+  (S : Set α) :
+  Set α :=
   {y | ∃ x, x ∈ S ∧ (x, y) ∈ r}
 
 
@@ -489,6 +491,17 @@ lemma reachable_closed_dfs
     obtain s1 := next_subset_dfs g stack []
     have s2 : reachable g stack ⊆ reachable g (dfs_aux g stack []) := reachable_mono g stack (dfs_aux g stack []) s1
 
+    have s2_5 : reachable g (dfs_aux g stack []) = (dfs_aux g stack []).toFinset.toSet :=
+    by
+      obtain s3 := nextss_closed_dfs g stack
+      simp only [nextss] at s3
+
+      have s4 : relation_image g.toFinset.toSet (dfs_aux g stack []).toFinset.toSet ⊆ (dfs_aux g stack []).toFinset.toSet :=
+      by
+        simp only [relation_image]
+        aesop
+      simp only [relation_image] at s4
+      sorry
     sorry
 
 
